VCVio/OracleComp/SimSemantics/Simulate.lean
@@ -170,7 +170,6 @@ lemma simulate_eq_map_simulate'_of_subsingleton [Subsingleton σ] (oa : OracleCo
   simp only [simulate', map_eq_bind_pure_comp, bind_assoc, Function.comp_apply, pure_bind]
   convert symm (bind_pure (simulate so oa s))
 
-@[simp]
 lemma simulate_eq_map_simulate' [Subsingleton σ] [Inhabited σ] (oa : OracleComp spec α)
     (s : σ) : simulate so oa s = (·, default) <$> simulate' so oa s :=
   simulate_eq_map_simulate'_of_subsingleton so oa s default
